src/simulation/CertExecution2.v
@@ -391,17 +391,73 @@ constructor.
 Qed.
 
 Lemma cert_complete : complete certG.
-Proof using TCCOH WF WF_SC IT_new_co SAME ST_in_E S_in_W COMP_C COMP_NTID COMP_PPO COMP_RPPO.
+Proof using All.
   unfold complete; ins.
   rewrite cert_R, cert_E.
-  unfolder; ins; desf.
-  destruct (classic (D x)).
-  { forward (eapply (complete_D) with (T:=T) (x:=x)); try edone.
+  unfold Cert_rf.cert_rf.
+  arewrite (E ∩₁ R ⊆₁ E ∩₁ R ∩₁ D ∪₁ 
+                      E ∩₁ R ∩₁ set_compl (dom_rel Grmw) ∩₁ set_compl D ∪₁ 
+                      E ∩₁ R ∩₁ (dom_rel Grmw) ∩₁ set_compl D).
+  { unfolder; ins; desf. 
+    destruct (classic (D x)); destruct (classic ((dom_rel Grmw) x)); eauto 10. }
+unionL.
+{ unfolder; ins; desf.
+forward (eapply (complete_D) with (T:=T) (x:=x)); try edone.
     unfold Cert_rf.cert_rf.
     unfolder; ins; desf; eauto 20. }
-  admit.
-  (* forward (apply new_rf_comp); try edone. *)
-  (* unfold Cert_rf.cert_rf; basic_solver 12. *)
-Admitted.
+{ unfolder; ins; desf.
+forward (apply new_rf_comp); try edone. 
+  unfold Cert_rf.cert_rf; basic_solver 12. }
+
+
+
+
+unfolder; ins; desf.
+
+forward (eapply (@fsupp_immediate_pred _ Cco) with (x:=y)).
+{ eapply fsupp_mon; [| eapply fsupp_cross].
+apply dom_helper_3.
+eapply WF_cert.
+unfold acts_set.
+unfold set_finite.
+eauto. }
+
+{ eapply WF_cert.(co_irr). }
+{ eapply WF_cert.(co_trans). }
+{ unfolder; intro HH.
+apply WF_cert.(wf_rmwD) in H1; unfolder in H1; desf.
+apply WF_cert.(wf_rmwE) in H3; unfolder in H3; desf.
+exploit is_w_loc; eauto; ins; desf.
+ eapply HH with (b := InitEvent l).
+
+eapply tot_ex.
+- eapply WF_cert.
+- basic_solver.
+- unfolder; splits; try edone.
+  eapply (wf_init WF_cert); exists y; splits; eauto.
+by unfold is_w;
+  rewrite (wf_init_lab WF_cert) in *.
+rewrite x1.
+by unfold loc; rewrite (wf_init_lab WF_cert) in *.
+- intro A.
+eapply cert_co_sb_irr with (T:=T); eauto.
+unfolder; eexists; splits; eauto.
+eapply init_ninit_sb with (G:=certG); eauto.
+by apply WF_cert.
+by apply (wf_init WF_cert); eexists; splits; eauto.
+
+eapply WF_cert.(rmw_non_init_lr) in H5; unfolder in H5; desf.
+- 
+intro. 
+eapply WF_cert.(rmw_non_init_lr) in H5; unfolder in H5; desf.
+}
+
+unfolder; ins ;desf.
+
+eexists; eauto.
+right.
+eexists; split; eauto.
+Qed.
+
 
 End CertExec.
